compiler/dsl/coq/ReflexIO.v
@@ -13,13 +13,13 @@ Require Import ReflexBase.
 Ltac sep' := sep fail idtac.
 
 Inductive Action : Set :=
-| Exec   : Str -> list Str -> FD -> Action
-| Call   : Str -> list Str -> FD -> Action
-| Select : list FD -> FD -> Action
-| Recv   : FD -> Str -> Action
-| Send   : FD -> Str -> Action
-| RecvFD : FD -> FD -> Action (* RecvFD f f' : use f to recv f' *)
-| SendFD : FD -> FD -> Action (* SendFD f f' : use f to send f' *)
+| Exec   : str -> list str -> fd -> Action
+| Call   : str -> list str -> fd -> Action
+| Select : list fd -> fd -> Action
+| Recv   : fd -> str -> Action
+| Send   : fd -> str -> Action
+| RecvFD : fd -> fd -> Action (* RecvFD f f' : use f to recv f' *)
+| SendFD : fd -> fd -> Action (* SendFD f f' : use f to send f' *)
 .
 
 Definition Trace : Set := list Action.
@@ -35,88 +35,88 @@ Definition ExecPerms : list Perm :=
 Definition CallPerms : list Perm :=
   RecvP :: RecvFDP :: nil.
 
-Axiom open : FD -> list Perm -> hprop.
+Axiom open : fd -> list Perm -> hprop.
 
 Axiom exec :
-  forall (prog : Str) (args : list Str) (tr : [Trace]),
+  forall (prog : str) (args : list str) (tr : [Trace]),
     STsep (tr ~~ traced tr)
-          (fun f : FD => tr ~~ open f ExecPerms * traced (Exec prog args f :: tr)).
+          (fun f : fd => tr ~~ open f ExecPerms * traced (Exec prog args f :: tr)).
 
 Axiom call :
-  forall (prog : Str) (args : list Str) (tr : [Trace]),
+  forall (prog : str) (args : list str) (tr : [Trace]),
   STsep (tr ~~ traced tr)
-        (fun f : FD => tr ~~ open f CallPerms * traced (Call prog args f :: tr)).
+        (fun f : fd => tr ~~ open f CallPerms * traced (Call prog args f :: tr)).
 
 (* TODO add non-empty precondition *)
 (* TODO add open w/ recv perms precondition *)
 Axiom select :
-  forall (fs : list FD) (tr : [Trace]),
+  forall (fs : list fd) (tr : [Trace]),
   STsep (tr ~~ traced tr)
-        (fun f : FD => tr ~~ traced (Select fs f :: tr) * [In f fs]).
+        (fun f : fd => tr ~~ traced (Select fs f :: tr) * [In f fs]).
 
 Axiom recv :
-  forall (f : FD) (ps : list Perm) (n : Num) (tr : [Trace]),
+  forall (f : fd) (ps : list Perm) (n : num) (tr : [Trace]),
   STsep (tr ~~ traced tr * open f ps * [In RecvP ps])
-        (fun s : Str => tr ~~ traced (Recv f s :: tr) * open f ps *
-          [nat_of_Num n = List.length s]).
+        (fun s : str => tr ~~ traced (Recv f s :: tr) * open f ps *
+          [nat_of_num n = List.length s]).
 
 Axiom send :
-  forall (f : FD) (ps : list Perm) (s : Str) (tr : [Trace]),
+  forall (f : fd) (ps : list Perm) (s : str) (tr : [Trace]),
   STsep (tr ~~ traced tr * open f ps * [In SendP ps])
         (fun _ : unit => tr ~~ traced (Send f s :: tr) * open f ps).
 
 Axiom recv_fd :
-  forall (f : FD) (ps : list Perm) (tr : [Trace]),
+  forall (f : fd) (ps : list Perm) (tr : [Trace]),
   STsep (tr ~~ traced tr * open f ps * [In RecvFDP ps])
-        (fun f' : FD => tr ~~ traced (RecvFD f f' :: tr) * open f ps).
+        (fun f' : fd => tr ~~ traced (RecvFD f f' :: tr) * open f ps).
 
 Axiom send_fd :
-  forall (f : FD) (ps : list Perm) (f' : FD) (tr : [Trace]),
+  forall (f : fd) (ps : list Perm) (f' : fd) (tr : [Trace]),
   STsep (tr ~~ traced tr * open f ps * [In SendFDP ps])
         (fun _ : unit => tr ~~ traced (SendFD f f' :: tr) * open f ps).
 
 (* we use big endian to follow network order *)
-Definition RecvNum (f : FD) (n : Num) : Trace :=
+Definition RecvNum (f : fd) (n : num) : Trace :=
   match n with
-  | num l h => Recv f (h :: l :: nil) :: nil
+  | Num l h => Recv f (h :: l :: nil) :: nil
   end.
 
-Definition SendNum (f : FD) (n : Num) : Trace :=
+Definition SendNum (f : fd) (n : num) : Trace :=
   match n with
-  | num l h => Send f (h :: l :: nil) :: nil
+  | Num l h => Send f (h :: l :: nil) :: nil
   end.
 
-Definition RecvStr (f : FD) (s : Str) : Trace :=
-  Recv f s :: RecvNum f (Num_of_nat (List.length s)).
+Definition RecvStr (f : fd) (s : str) : Trace :=
+  Recv f s :: RecvNum f (num_of_nat (List.length s)).
 
-Definition SendStr (f : FD) (s : Str) : Trace :=
-  Send f s :: SendNum f (Num_of_nat (List.length s)).
+Definition SendStr (f : fd) (s : str) : Trace :=
+  Send f s :: SendNum f (num_of_nat (List.length s)).
 
 Definition recv_num:
-  forall (f : FD) (ps : list Perm) (tr : [Trace]),
+  forall (f : fd) (ps : list Perm) (tr : [Trace]),
   STsep (tr ~~ traced tr * open f ps * [In RecvP ps])
-        (fun n : Num => tr ~~ traced (RecvNum f n ++ tr) * open f ps).
+        (fun n : num => tr ~~ traced (RecvNum f n ++ tr) * open f ps).
 Proof.
   intros; refine (
-    s <- recv f ps (num "002" "000") tr;
+    s <- recv f ps (Num "002" "000") tr;
     match s with
     | h :: l :: nil =>
-      {{ Return (num l h) }}
+      {{ Return (Num l h) }}
     | _ => (* bogus *)
-      {{ Return (num "000" "000") }}
+      {{ Return (Num "000" "000") }}
     end
   );
   sep'; discriminate.
 Qed.
 
 Definition send_num:
-  forall (f : FD) (ps : list Perm) (n : Num) (tr : [Trace]),
+  forall (f : fd) (ps : list Perm) (n : num) (tr : [Trace]),
   STsep (tr ~~ traced tr * open f ps * [In SendP ps])
         (fun _ : unit => tr ~~ traced (SendNum f n ++ tr) * open f ps).
 Proof.
   intros; refine (
     match n with
-    | num l h =>
+    | Num l h =>
       send f ps (h :: l :: nil) tr;;
       {{ Return tt }}
     end
@@ -125,9 +125,9 @@ Proof.
 Qed.
 
 Definition recv_str:
-  forall (f : FD) (ps : list Perm) (tr : [Trace]),
+  forall (f : fd) (ps : list Perm) (tr : [Trace]),
   STsep (tr ~~ traced tr * open f ps * [In RecvP ps])
-        (fun s : Str => tr ~~ traced (RecvStr f s ++ tr) * open f ps).
+        (fun s : str => tr ~~ traced (RecvStr f s ++ tr) * open f ps).
 Proof.
   intros; refine (
     n <- recv_num f ps tr <@> [In RecvP ps];
@@ -136,17 +136,17 @@ Proof.
   );
   sep'.
   rewrite <- H.
-  rewrite Num_nat_embedding.
+  rewrite num_nat_embedding.
   sep'.
 Qed.
 
 Definition send_str:
-  forall (f : FD) (ps : list Perm) (s : Str) (tr : [Trace]),
+  forall (f : fd) (ps : list Perm) (s : str) (tr : [Trace]),
   STsep (tr ~~ traced tr * open f ps * [In SendP ps])
         (fun (_ : unit) => tr ~~ traced (SendStr f s ++ tr) * open f ps).
 Proof.
   intros; refine (
-    let n := Num_of_nat (List.length s) in
+    let n := num_of_nat (List.length s) in
     send_num f ps n tr <@> [In SendP ps];;
     send f ps s (tr ~~~ SendNum f n ++ tr);;
     {{ Return tt }}
@@ -157,20 +157,20 @@ Qed.
 (* prevent sep tactic from unfolding *)
 Global Opaque RecvNum SendNum RecvStr SendStr.
 
-Definition bound (f : FD) : hprop :=
+Definition bound (f : fd) : hprop :=
   open f ExecPerms.
 
-Fixpoint all_bound (fds : list FD) : hprop :=
+Fixpoint all_bound (fds : list fd) : hprop :=
   match fds with
   | nil => emp
   | f :: fs => bound f * all_bound fs
   end.
 
-Fixpoint all_bound_drop (fds : list FD) (drop : FD) : hprop :=
+Fixpoint all_bound_drop (fds : list fd) (drop : fd) : hprop :=
   match fds with
   | nil => emp
   | f :: fs =>
-    if FD_eq f drop
+    if fd_eq f drop
       then all_bound fs
       else bound f * all_bound_drop fs drop
   end.
@@ -181,8 +181,8 @@ Lemma unpack_all_bound :
   all_bound fs ==> bound f * all_bound_drop fs f.
 Proof.
   induction fs; simpl; intros. contradiction.
-  destruct H; subst. rewrite FD_eq_true. apply himp_refl.
-  case (FD_eq a f); intros; subst. apply himp_refl.
+  destruct H; subst. rewrite fd_eq_true. apply himp_refl.
+  case (fd_eq a f); intros; subst. apply himp_refl.
   apply himp_comm_conc. apply himp_assoc_conc1.
   apply himp_split. apply himp_refl.
   apply himp_comm_conc; auto.
@@ -194,8 +194,8 @@ Lemma repack_all_bound :
   bound f * all_bound_drop fs f ==> all_bound fs.
 Proof.
   induction fs; simpl; intros. contradiction.
-  destruct H; subst. rewrite FD_eq_true. apply himp_refl.
-  case (FD_eq a f); intros; subst. apply himp_refl.
+  destruct H; subst. rewrite fd_eq_true. apply himp_refl.
+  case (fd_eq a f); intros; subst. apply himp_refl.
   apply himp_comm_prem. apply himp_assoc_prem1.
   apply himp_split. apply himp_refl.
   apply himp_comm_prem; auto.
